proof/invariant-abstract/ARM/ArchAcc_AI.thy
@@ -317,15 +317,14 @@ lemma mask_asid_low_bits_ucast_ucast:
 
 
 lemma set_asid_pool_cur [wp]:
-  "\<lbrace>\<lambda>s. P (cur_thread s)\<rbrace> set_asid_pool p a \<lbrace>\<lambda>_ s. P (cur_thread s)\<rbrace>"
+  "\<lbrace>\<lambda>s. P (cur_thread s)\<rbrace> do_extended_op (set_asid_pool p a) \<lbrace>\<lambda>_ s. P (cur_thread s)\<rbrace>"
   unfolding set_asid_pool_def by (wpsimp wp: get_object_wp)
 
 
 lemma set_asid_pool_cur_tcb [wp]:
-  "\<lbrace>\<lambda>s. cur_tcb s\<rbrace> set_asid_pool p a \<lbrace>\<lambda>_ s. cur_tcb s\<rbrace>"
+  "\<lbrace>\<lambda>s. cur_tcb s\<rbrace> do_extended_op (set_asid_pool p a) \<lbrace>\<lambda>_ s. cur_tcb s\<rbrace>"
   unfolding cur_tcb_def
-  by (rule hoare_lift_Pf [where f=cur_thread]; wp)
-
+  by (rule hoare_lift_Pf [where f=cur_thread]; wpsimp)
 
 crunch arch [wp]: set_asid_pool "\<lambda>s. P (arch_state s)"
   (wp: get_object_wp)
@@ -926,13 +925,6 @@ lemma set_pd_reply_caps:
   by (wp valid_reply_caps_st_cte_lift)
 
 
-lemma set_pd_reply_masters:
-  "\<lbrace>valid_reply_masters\<rbrace>
-   set_pd p pd
-   \<lbrace>\<lambda>_. valid_reply_masters\<rbrace>"
-  by (wp valid_reply_masters_cte_lift)
-
-
 lemma global_refs_kheap [simp]:
   "global_refs (kheap_update f s) = global_refs s"
   by (simp add: global_refs_def)
@@ -1079,10 +1071,6 @@ lemma set_pt_ifunsafe:
 lemma set_pt_reply_caps:
   "\<lbrace>\<lambda>s. valid_reply_caps s\<rbrace> set_pt p pt \<lbrace>\<lambda>_ s. valid_reply_caps s\<rbrace>"
   by (wp valid_reply_caps_st_cte_lift)
-
-lemma set_pt_reply_masters:
-  "\<lbrace>valid_reply_masters\<rbrace>  set_pt p pt  \<lbrace>\<lambda>_. valid_reply_masters\<rbrace>"
-  by (wp valid_reply_masters_cte_lift)
 
 
 crunch global_ref [wp]: set_pt "\<lambda>s. P (global_refs s)"
@@ -1624,11 +1612,11 @@ lemma set_pt_invs:
    \<lbrace>\<lambda>_. invs\<rbrace>"
   apply (simp add: invs_def valid_state_def valid_pspace_def)
   apply (rule hoare_pre)
-   apply_trace (wp set_pt_valid_objs set_pt_iflive set_pt_zombies
+   apply (wp set_pt_valid_objs set_pt_iflive set_pt_zombies
              set_pt_zombies_state_refs set_pt_zombies_state_hyp_refs set_pt_valid_mdb
              set_pt_valid_idle set_pt_ifunsafe set_pt_reply_caps
              set_pt_valid_arch_state set_pt_valid_global set_pt_cur
-             set_pt_reply_masters valid_irq_node_typ
+             valid_irq_node_typ
              valid_irq_handlers_lift
              set_pt_valid_global_vspace_mappings)
   apply (clarsimp dest!: valid_objs_caps)
@@ -1839,13 +1827,6 @@ lemma set_asid_pool_reply_caps [wp]:
   set_asid_pool p ap
   \<lbrace>\<lambda>_ s. valid_reply_caps s\<rbrace>"
   by (wp valid_reply_caps_st_cte_lift)
-
-
-lemma set_asid_pool_reply_masters [wp]:
-  "\<lbrace>valid_reply_masters\<rbrace>
-   set_asid_pool p ap
-   \<lbrace>\<lambda>_. valid_reply_masters\<rbrace>"
-  by (wp valid_reply_masters_cte_lift)
 
 
 crunch global_ref [wp]: set_asid_pool "\<lambda>s. P (global_refs s)"
@@ -2110,19 +2091,22 @@ lemma set_asid_pool_vms[wp]:
                   split: kernel_object.splits arch_kernel_obj.splits)+
   done
 
+lemma cur_tcb_more_update[iff]:
+  "cur_tcb (trans_state f s) = cur_tcb s"
+  by (simp add: cur_tcb_def)
 
 lemma set_asid_pool_invs_restrict:
   "\<lbrace>invs and ko_at (ArchObj (ASIDPool ap)) p and
     (\<lambda>s. \<forall>asid. asid \<le> mask asid_bits \<longrightarrow> ucast asid \<notin> S \<longrightarrow>
                 arm_asid_table (arch_state s) (asid_high_bits_of asid) = Some p \<longrightarrow>
                 arm_asid_map (arch_state s) asid = None)\<rbrace>
-       set_asid_pool p (ap |` S) \<lbrace>\<lambda>_. invs\<rbrace>"
+       do_extended_op (set_asid_pool p (ap |` S)) \<lbrace>\<lambda>_. invs\<rbrace>"
   apply (simp add: invs_def valid_state_def valid_pspace_def
                    valid_arch_caps_def)
   apply (wp valid_irq_node_typ set_asid_pool_typ_at
             set_asid_pool_vspace_objs_unmap  valid_irq_handlers_lift
             set_asid_pool_vs_lookup_unmap set_asid_pool_restrict_asid_map)
-  apply simp
+  apply simp_all
   done
 
 
@@ -2144,7 +2128,7 @@ lemma set_asid_pool_invs_unmap:
     (\<lambda>s. \<forall>asid. asid \<le> mask asid_bits \<longrightarrow> ucast asid = x \<longrightarrow>
                 arm_asid_table (arch_state s) (asid_high_bits_of asid) = Some p \<longrightarrow>
                 arm_asid_map (arch_state s) asid = None)\<rbrace>
-       set_asid_pool p (ap(x := None)) \<lbrace>\<lambda>_. invs\<rbrace>"
+       do_extended_op (set_asid_pool p (ap(x := None))) \<lbrace>\<lambda>_. invs\<rbrace>"
   using set_asid_pool_invs_restrict[where S="- {x}"]
   by (simp add: restrict_map_def fun_upd_def if_flip)
 
@@ -3250,7 +3234,7 @@ lemma set_pd_invs_unmap:
              set_pd_zombies_state_refs set_pd_valid_mdb
              set_pd_valid_idle set_pd_ifunsafe set_pd_reply_caps
              set_pd_valid_arch set_pd_valid_global set_pd_cur
-             set_pd_reply_masters valid_irq_node_typ set_pd_zombies_state_hyp_refs
+             valid_irq_node_typ set_pd_zombies_state_hyp_refs
              set_pd_vspace_objs_unmap set_pd_vs_lookup_unmap
              valid_irq_handlers_lift
              set_pd_unmap_mappings set_pd_equal_kernel_mappings_triv)
