proof/invariant-abstract/ARM/ArchInvariants_AI.thy
@@ -2381,6 +2381,7 @@ lemma hyp_live_tcb_simps[simp]:
 "\<And>tcb f. hyp_live (TCB (tcb_ipcframe_update f tcb)) = hyp_live (TCB tcb)"
 "\<And>tcb f. hyp_live (TCB (tcb_state_update f tcb)) = hyp_live (TCB tcb)"
 "\<And>tcb f. hyp_live (TCB (tcb_fault_handler_update f tcb)) = hyp_live (TCB tcb)"
+"\<And>tcb f. hyp_live (TCB (tcb_timeout_handler_update f tcb)) = hyp_live (TCB tcb)"
 "\<And>tcb f. hyp_live (TCB (tcb_fault_update f tcb)) = hyp_live (TCB tcb)"
 "\<And>tcb f. hyp_live (TCB (tcb_bound_notification_update f tcb)) = hyp_live (TCB tcb)"
   by (simp_all add: hyp_live_tcb_def)
